examples/priority_queue/PQueueA.v
@@ -1,0 +1,197 @@
+Require Import CRIS.
+Require Import MemHeader MemA MemTactics.
+Require Import SchHeader SchI SchA SchTactics.
+Require Import StackHeader StackA.
+Require Import PQueueHeader PQueueI.
+From iris.algebra Require Import excl_auth.
+
+Class queueG `{!crisG Γ Σ α β τ _S _I} := QueueG {
+  queue_stateG :: inG (excl_authR (listO (leibnizO (val * gname)))) Γ;
+}.
+Definition queueΓ : HRA := #[excl_authR (listO (leibnizO (val * gname)))].
+Global Instance subG_queueG `{!crisG Γ Σ α β τ _S _I} :
+  subG queueΓ Γ → queueG.
+Proof. solve_inG. Defined.
+Hint Unfold subG_queueG queue_stateG : GRA_index.
+
+Section definitions.
+  Context `{!crisG Γ Σ α β τ _S _I, !concG, !newschG, !memG}.
+  Context `{!stackG StackM.jobID StackM.retID, !queueG}.
+  Context (N : namespace).
+
+  Definition queueN : namespace := N.@"queue".
+
+  Definition syn_queue_inv
+      (n : nat) (γq : gname) (range : nat) (qb : mblock) (qofs : ptrofs)
+      (entries : list (leibnizO (val * gname)))
+      : GTerm.t n := (
+    <own> γq (excl_auth_frag entries) ∗
+    [∗ n list] i ↦ x ∈ entries, (qb, qofs + i)%Z ↦ x.1
+  )%SAT.
+  Definition queue_inv
+      (n : nat) (γq : gname) (range : nat) (qb : mblock) (qofs : ptrofs) 
+      (entries : list (leibnizO (val * gname)))
+      : iProp Σ := (
+    own γq (◯E entries) ∗
+    [∗ list] i ↦ x ∈ entries, (qb, qofs + Z.of_nat i)%Z ↦ x.1
+  )%I.
+  Global Instance queue_inv_SLRed n γq range qb qofs entries :
+    SLRed (syn_queue_inv n γq range qb qofs entries) (queue_inv n γq range qb qofs entries).
+  Proof. rewrite /syn_queue_inv /queue_inv; econs; rewrite SLRed_eq //. Qed.
+
+  Definition syn_is_queue (n : nat) (γq : gname) (range : nat) (q : val) : GTerm.t n := (
+    ∃ (qb : τ{mblock}) (qofs : τ{ptrofs}), ⌜q = Vptr (qb, qofs)⌝ ∗
+      ∃ (entries : τ{list (val * gname)}),
+        syn_inv n queueN (syn_queue_inv n γq range qb qofs entries) ∗
+        [∗ n list] i ↦ e ∈ entries, syn_is_stack (stackN N) e.2 e.1 n
+  )%SAT.
+  Definition is_queue (n : nat) (γq : gname) (range : nat) (q : val) : iProp Σ :=
+    ∃ (qb : mblock) (qofs : ptrofs), ⌜q = Vptr (qb, qofs)⌝ ∗
+      ∃ (entries : list (val * gname)),
+        inv n queueN (syn_queue_inv n γq range qb qofs entries) ∗
+        [∗ list] i ↦ e ∈ entries, is_stack (stackN N) e.2 e.1 n.
+  Global Instance is_queue_SLRed n γq q range :
+    SLRed (syn_is_queue n γq q range) (is_queue n γq q range).
+  Proof.
+    rewrite /syn_is_queue /is_queue; econs; rewrite SLRed_eq //. do 4 (f_equiv; ii); ss.
+    rewrite inv_red //.
+  Qed.
+  Global Instance is_queue_persistent n γq q range :
+    Persistent (is_queue n γq q range).
+  Proof. apply _. Qed.
+
+  Definition queue_contents (γq : gname) (range : nat) (map : list (list val)) : iProp Σ :=
+    ∃ (entries : list (leibnizO (val * gname))), own γq (●E entries) ∗
+      [∗ list] i ↦ e ∈ entries, stack_content e.2 (map !!! i).
+End definitions.
+
+Module PQueueA. Section PQueueA.
+  Context `{!crisG Γ Σ α β τ _S _I, !concG, !newschG, !memG}.
+  Context `{!stackG StackM.jobID StackM.retID, !queueG}.
+  Context (N : namespace).
+
+  Definition scopes : list string := [].
+
+  Definition new_spec : fspec :=
+    fspec_sch (↑N)
+      (fspec_simple (X := nat * nat) (λ '(n, range),
+        ((λ arg, ⌜arg = [Vint range]↑ ∧ 8 * range < modulus_64⌝)%Z,
+         (λ ret, ∃ q γq, ⌜ret = q↑⌝ ∗
+          is_queue N n γq range q ∗ queue_contents γq range (repeat [] range)))%I)).
+
+  Definition new : Any.t → itree crisE Any.t := λ _,
+    𝒴;;; fbody_trivial ()↑.
+
+  Definition fnsems : fnsems_type :=
+    [(Some PQueueHdr.new, (true, wmask_all, scopes, (Some new_spec, new)))].
+
+  Program Definition Mod : SMod.t := {|
+    SMod.scopes := scopes;
+    SMod.fnsems := fnsems;
+    SMod.initial_st := [];
+  |}.
+  Solve All Obligations with prove_scope.
+  Next Obligation. prove_nodup. Qed.
+
+  Definition t sp := Seal.sealing CRIS (SMod.to_mod sp Mod).
+End PQueueA. End PQueueA.
+
+Module PQueueIA. Section PQueueIA.
+  Context `{!crisG Γ Σ α β τ _S _I, !concG, !newschG, !memG}.
+  Context `{!stackG StackM.jobID StackM.retID, !queueG}.
+
+  Context (N : namespace) (sp : sp_type).
+  Context (Hsch : sp_incl (SchA.sp [] (↑N)) sp).
+
+  Definition init_cond : iProp Σ := emp%I.
+
+  Local Definition PQueueI := PQueueI.t      ★ StackA.t N sp ★ SchI.t ★ MemA.t.
+  Local Definition PQueueA := PQueueA.t N sp ★ StackA.t N sp ★ SchI.t ★ MemA.t.
+  Local Definition IstFull := IstProd (IstSB (Mod.scopes (PQueueA.t N sp)) IstTrue) IstEq.
+
+  Lemma new_simF : ISim.sim_fun open PQueueA PQueueI init_cond IstFull (Some PQueueHdr.new).
+  Proof.
+    init_simF.
+    steps_l. iDestruct "ASM" as "[TID [[-> %Hn] ->]]".
+    rename _q3 into stid, _q4 into mtid, _q5 into n, _q6 into range.
+
+    steps_r. hss_r. steps_r. sch_yield_ir. steps_r. sch_yield_ir. steps_r.
+    iApply wsim_mem_alloc; [try prove_inline_cond|try prove_sb_cond|ss|unfold_cris_defs].
+    { lia. }
+    iIntros (queueb) "↦queue". steps_r. hss_r. steps_r. sch_yield_ir. steps_r.
+
+    iApply wsim_yy_y. iApply wsim_bind.
+    instantiate (1:=(λ '(st_src, _) '(st_tgt, _),
+      IstFull st_src st_tgt ∗ Tid stid mtid ∗ winv (↑N, ↑N) ∗
+      ∃ γq, is_queue N n γq range (Vptr (queueb, 0%Z)) ∗
+      queue_contents γq range (repeat [] range))%I).
+    iSplitL "↦queue IST TID".
+    { rewrite ?Nat2Z.id. erewrite <-(bind_ret_r (SB.sandbox _ _ _ _)).
+      iAssert ([∗ list] i ↦ v ∈ repeat Vundef range,
+        if (decide (0%Z ≤ i)%Z)
+        then (queueb, Z.of_nat i) ↦ v
+        else ∃ γs stack, is_stack N γs stack n ∗ (queueb, Z.of_nat i) ↦ stack)%I
+        with "[↦queue]" as "↦queue".
+      { iApply (big_sepL_impl with "↦queue").
+        iIntros "!> % % %"; case_decide; try iIntros "$"; lia.
+      }
+      set (var := range).
+      rewrite {1 2 3 4}/var.
+      replace (0%Z) with (range - var)%Z by lia.
+      rewrite {5}Z.sub_diag.
+       (* rewrite {1 3 5 6 7 8 9 10 11 12 13 14 15 17}/var. *)
+      iAssert (⌜var ≤ range⌝)%I as "#Hvar"; first (iPureIntro; lia).
+      generalize var. clear var. iIntros (var).
+      iInduction (var) as [|var] forall (st_src st_tgt).
+      { unfold_iter_r. steps_r.
+        erewrite <-(bind_ret_r (SB.sandbox _ _ _ _)).
+        sch_yield_l. ss.
+        iMod (own_alloc (●E [] ⋅ ◯E [])) as "[%γq [●q ◯q]]"; first eauto using excl_auth_valid.
+        iMod (inv_alloc (syn_queue_inv n γq range queueb 0 []) _ _ _ (queueN N) with "[◯q]")
+          as "#Qinv"; eauto.
+        { apply nclose_subseteq. }
+        { rewrite SLRed_eq /queue_inv; iFrame; ss. }
+        iApply wsim_unfold; iIntros "W". step. iFrame "IST TID W". iExists γq. iSplitR "●q".
+        { iExists _, _; iSplit; first done; iExists []; ss; iSplit; iFrame; eauto. }
+        iExists _; iFrame; ss.
+      }
+
+      iPoseProof "Hvar" as "%".
+      unfold_iter_r. steps_r.
+      (* stack allocation *)
+      inline_r. force_r (stid, mtid, n). forces_r. iFrame. iSplit; eauto.
+      steps_r. hss_r. steps_r. steps_l. steps_r. sch_yield_ii.
+      steps_r. iDestruct "GRT" as "[TID [[%stack [%γs [-> [#is_stack stack]]]] %]]".
+      hss_r. steps_r.
+      iPoseProof (big_sepL_lookup_acc_impl (range - S var) Vundef with "↦queue")
+        as "[↦queue ↦close]".
+      { hexploit (lookup_lt_is_Some_2 (repeat Vundef range) (range - S var)).
+        { rewrite repeat_length. lia. }
+        destruct (repeat Vundef range !! _) eqn : Hlkn; ss; last (intros INV; inv INV).
+        apply elem_of_list_lookup_2, elem_of_list_In, repeat_spec in Hlkn; clarify.
+      }
+      case_decide; last lia.
+
+      iApply (wsim_mem_store with "[↦queue]");
+        [try prove_inline_cond|try prove_sb_cond|..|unfold_cris_defs].
+      { rewrite Nat2Z.inj_sub //. }
+      iIntros "↦queue". steps_r. hss_r. steps_r.
+      replace (range - S var + 1)%Z with (range - var)%Z by lia.
+      iApply ("IHvar" with "[] IST TID [-]").
+      { iIntros "!>"; iPureIntro; lia. }
+      iApply ("↦close" with "[] [↦queue]").
+      { iModIntro; iIntros (??) "%% H"; do 2 case_decide; try lia; iFrame. }
+      { case_decide; try lia.
+        iExists _, _; iFrame "is_stack". rewrite Nat2Z.inj_sub //; iFrame.
+      }
+    }
+
+    (* continuation *)
+    clear_st. iIntros (st_s _ st_t _) "[IST [TID [W [%γq [#qinv queue]]]]]".
+    iApply wsim_fold; iFrame "W".
+    steps_r. sch_yield_ir. steps_r.
+    sch_yield_l. forces_l. iFrame. iSplit; eauto. step. iSplit; done.
+  Unshelve. all: eauto.
+  (*SLOW*)Qed.
+End PQueueIA. End PQueueIA.
+
