examples/priority_queue/PQueueI.v
@@ -1,0 +1,46 @@
+Require Import CRIS.
+Require Import SchHeader.
+Require Import MemHeader.
+Require Import StackHeader.
+Require Import PQueueHeader.
+
+Module PQueueI. Section PQueueI.
+  Context `{!crisG Γ Σ α β τ _S _I, !concG}.
+
+  Definition scopes : list string := [].
+
+  Definition new : list val → itree crisE val := λ args,
+    𝒴;;; 'n : Z <- (pargs [Tint] args)?;;
+    𝒴;;; 'queue : val <- ccallU MemHdr.alloc [Vint n];;
+    𝒴;;; '(b, ofs) : _ <- (pargs [Tptr] [queue])?;;
+    let n := Z.to_nat n in
+    ITree.iter (λ '(n, ofs),
+      match n with
+      | 0 => Ret (inr ())
+      | S n' =>
+          'bin : val <- ccallU StackHdr.new_stack (@nil val);;
+          '_ : val <- ccallU MemHdr.store [Vptr (b, ofs); bin];; Ret (inl (n', (ofs + 1)%Z))
+      end
+    ) (n, ofs);;;
+    𝒴;;; Ret queue.
+
+  Definition add : list val → itree crisE val := λ args,
+    𝒴;;; '(queueb, queueofs, (p, v)) : _ <- (pargs [Tptr; Tint; Tuntyped] args)?;;
+    𝒴;;; 'bin : val <- ccallU MemHdr.load [Vptr (queueb, queueofs + p)%Z];;
+    𝒴;;; '_ : val <- ccallU StackHdr.push [bin; v];;
+    𝒴;;; Ret Vundef.
+
+  Definition fnsems : fnsems_type :=
+    [(Some PQueueHdr.new, (false, wmask_all, scopes, (None, cfunU new)));
+     (Some PQueueHdr.add, (false, wmask_all, scopes, (None, cfunU add)))].
+
+  Program Definition Mod : SMod.t := {|
+    SMod.scopes := scopes;
+    SMod.fnsems := fnsems;
+    SMod.initial_st := [];
+  |}.
+  Solve All Obligations with prove_scope.
+  Next Obligation. prove_nodup. Qed.
+
+  Definition t := Seal.sealing CRIS (SMod.to_mod sp_none Mod).
+End PQueueI. End PQueueI.
